SVAuth/AuthClassHierarchy/OAuth20.cs
@@ -8,6 +8,9 @@ using System.Threading.Tasks;
 using System.Diagnostics;
 using System.Collections.Generic;
 using System.Reflection;
+using System.Diagnostics.Contracts;
+using System.Security.Cryptography;
+using System.Text;
 
 namespace SVAuth.OAuth20
 {
@@ -16,40 +19,29 @@ namespace SVAuth.OAuth20
     /*               Messages between parties                  */
     /***********************************************************/
 
-    public class AuthorizationRequest : GenericAuth.SignInIdP_Req
+    public class AuthorizationRequest : SVX.SVX_MSG
     {
         public string response_type;
         public string client_id;
+#if false
         public override string Realm
         {
             get { return client_id; }
             set { client_id = value; }
         }
-        public string redirect_uri = null;
+#endif
+        public string redirect_uri;
         public string scope;
-        // Nothing references this.  Just remove it rather than exclude it from
-        // serialization? ~ t-mattmc@microsoft.com 2016-06-01
-        //public string state = null;
+        public SVX.Secret state;
     }
 
-    public class AuthorizationResponse : GenericAuth.SignInIdP_Resp_SignInRP_Req
+    public class AuthorizationResponse : SVX.SVX_MSG
     {
-        public string code;
-        public string state = null;
-
-        public AuthorizationResponse(AuthorizationResponse srcObj = null)
-        {
-            if (srcObj != null)
-            {
-                code = srcObj.code;
-                state = srcObj.state;
-                SymT = srcObj.SymT;
-                SignedBy = srcObj.SignedBy;
-            }
-        }
+        public SVX.Secret code;
+        public SVX.Secret state;
     }
 
-    public class AuthorizationErrorResponse : GenericAuth.SignInIdP_Resp_SignInRP_Req
+    public class AuthorizationErrorResponse : SVX.SVX_MSG
     {
         protected string error;
         protected string error_description = null;
@@ -60,15 +52,19 @@ namespace SVAuth.OAuth20
     public class AccessTokenRequest : SVX.SVX_MSG
     {
         public string grant_type;
-        public string code;
+        public SVX.Secret code;
         public string redirect_uri;
         public string client_id;
+        // Currently we do not model client_secret as an SVX secret because we
+        // do not need to reason about its secrecy.  We could still use an SVX
+        // secret if we wanted to make it harder to accidentally leak.
         public string client_secret;
         public string refresh_token = null;
     }
 
     public class AccessTokenResponse : SVX.SVX_MSG
     {
+        // Same remark as client_secret.
         public string access_token;
         public string token_type;
         public string expires_in;
@@ -83,11 +79,52 @@ namespace SVAuth.OAuth20
     public class UserProfileResponse : SVX.SVX_MSG
     {
     }
-    public class LoginResponse : GenericAuth.SignInRP_Resp
+#if false
+    public class LoginResponse
     {
         public string status;
     }
+#endif
 
+    [BCTOmit]
+    public class MessageStructures
+    {
+        // In many cases, we'll actually be using service-provider-specific
+        // message subclasses.  SVX will let us get away with this as long as
+        // the subclasses do not add any new secrets.  Maybe SVX should be
+        // stricter, but at the moment that would just cost us a lot of
+        // boilerplate for no practical benefit.
+        public readonly SVX.MessageStructure<AuthorizationRequest> authorizationRequest;
+        public readonly SVX.MessageStructure<AuthorizationResponse> authorizationResponse;
+        public readonly SVX.MessageStructure<AccessTokenRequest> accessTokenRequest;
+        public readonly SVX.MessageStructure<AccessTokenResponse> accessTokenResponse;
+        public readonly SVX.MessageStructure<UserProfileRequest> userProfileRequest;
+        public readonly SVX.MessageStructure<UserProfileResponse> userProfileResponse;
+
+        public MessageStructures(SVX.Principal idpPrincipal)
+        {
+            authorizationRequest = new SVX.MessageStructure<AuthorizationRequest> { BrowserOnly = true };
+            authorizationRequest.AddSecret(nameof(AuthorizationRequest.state),
+                (msg) => new SVX.PrincipalHandle[] { GenericAuth.GenericAuthStandards.GetUrlTargetPrincipal(msg.redirect_uri) });
+
+            authorizationResponse = new SVX.MessageStructure<AuthorizationResponse> { BrowserOnly = true };
+            authorizationResponse.AddSecret(nameof(AuthorizationResponse.state),
+                (msg) => new SVX.PrincipalHandle[] { });
+            authorizationResponse.AddSecret(nameof(AuthorizationResponse.code),
+                (msg) => new SVX.PrincipalHandle[] { idpPrincipal });
+
+            accessTokenRequest = new SVX.MessageStructure<AccessTokenRequest>();
+            accessTokenRequest.AddSecret(nameof(AccessTokenRequest.code),
+                (msg) => new SVX.PrincipalHandle[] { });
+
+            accessTokenResponse = new SVX.MessageStructure<AccessTokenResponse>();
+
+            userProfileRequest = new SVX.MessageStructure<UserProfileRequest>();
+            userProfileResponse = new SVX.MessageStructure<UserProfileResponse>();
+        }
+    }
+
+#if false
     /***********************************************************/
     /*               Data structures on parties                */
     /***********************************************************/
@@ -107,14 +144,6 @@ namespace SVAuth.OAuth20
         public string scope;
     }
 
-    public abstract class ID_Claim : GenericAuth.ID_Claim
-    {
-        string redirect_uri;
-        public override string Redir_dest
-        {
-            get { return redirect_uri; }
-        }
-    }
     /*
     public interface AuthorizationCodeRecs : GenericAuth.IdPAuthRecords_Base
     {
@@ -127,127 +156,183 @@ namespace SVAuth.OAuth20
         string findISSByClientIDAndRefreshToken(string client_id, string refresh_token);
     }
     */
-    // For interim use testing SVX_OPS.  Obviously this won't pass verification.
-    // ~ t-mattmc@microsoft.com 2016-06-07
-    public class DummyConcreteAuthorizationServer : GenericAuth.AS
-    {
-        public SVX.SVX_MSG DummyGetAccessToken(SVX.SVX_MSG input)
-        {
-            return new SVX.SVX_MSG();
-        }
-        public SVX.SVX_MSG DummyGetUserProfile(SVX.SVX_MSG input)
-        {
-            return new SVX.SVX_MSG();
-        }
-
-        public override GenericAuth.ID_Claim Process_SignInIdP_req(GenericAuth.SignInIdP_Req req)
-        {
-            throw new NotImplementedException();
-        }
-
-        public override GenericAuth.SignInIdP_Resp_SignInRP_Req Redir(string dest, GenericAuth.ID_Claim _ID_Claim)
-        {
-            throw new NotImplementedException();
-        }
-    }
+#endif
 
     /***********************************************************/
     /*                          Parties                        */
     /***********************************************************/
+
+    class StateParams
+    {
+        // Set an arbitrary fixed order to try to make sure the serialized form
+        // is reproducible.  It would matter in the middle of an upgrade of a
+        // replicated RP to a new .NET version that changes the field order
+        // returned by reflection.  Are there other reproducibility issues with
+        // Json.NET?
+
+        // We expect this to be a facet issued by the RP.
+        [JsonProperty(Order = 0)]
+        public SVX.PrincipalHandle client;
+
+        [JsonProperty(Order = 1)]
+        public SVX.Principal idpPrincipal;
+    }
+
+    // This class demonstrates how to use an HMAC, which is the easiest,
+    // especially for a replicated RP.  It might be better to use a dictionary
+    // (or an external key-value store) to enforce that each state is used only
+    // once and enforce an expiration time, etc.
+    class StateGenerator : SVX.SecretGenerator<StateParams>
+    {
+        readonly SVX.Principal rpPrincipal;
+        readonly string key;
+
+        // TODO: Get the key lazily once SVX supports the "prod context".
+        internal StateGenerator(SVX.Principal rpPrincipal, string key)
+        {
+            this.rpPrincipal = rpPrincipal;
+            this.key = key;
+        }
+
+        protected override SVX.PrincipalHandle[] GetReaders(object theParams)
+        {
+            var params2 = (StateParams)theParams;
+            return new SVX.PrincipalHandle[] { params2.idpPrincipal, rpPrincipal, params2.client };
+        }
+
+        protected override string RawGenerate(StateParams theParams)
+        {
+            return Utils.Hmac(JsonConvert.SerializeObject(theParams), key);
+        }
+
+        protected override void RawVerify(StateParams theParams, string secretValue)
+        {
+            if (secretValue != RawGenerate(theParams))
+                throw new ArgumentException();
+        }
+    }
+
     public abstract class Client : GenericAuth.RP
     {
+        // Lazy to avoid running initialization code in the vProgram.
+        MessageStructures messageStructures_;
+        MessageStructures messageStructures
+        {
+            get
+            {
+                if (messageStructures_ == null)
+                    messageStructures_ = new MessageStructures(idpParticipantId.principal);
+                return messageStructures_;
+            }
+        }
+
         public string client_id;
+#if false
         public override string Realm
         {
             get { return client_id; }
             set { client_id = value; }
         }
+#endif
         public string client_secret;
         public string TokenEndpointUrl;
         public string AuthorizationEndpointUrl;
         public string redirect_uri;
+#if false
         public override string Domain
         {
             get { return redirect_uri; }
             set { redirect_uri = value; }
         }
+#endif
+        internal StateGenerator stateGenerator;
+
         // Why are the parameters optional?  I don't see how this class can work without them. ~ t-mattmc@microsoft.com 2016-05-31
-        public Client(string client_id1 = null, string redierct_uri1 = null, string client_secret1 = null, string AuthorizationEndpointUrl1 = null, string TokenEndpointUrl1 = null)
+        public Client(SVX.Principal rpPrincipal,
+            string client_id1 = null, string redierct_uri1 = null, string client_secret1 = null,
+            string AuthorizationEndpointUrl1 = null, string TokenEndpointUrl1 = null,
+            string stateKey = null)
+            : base(rpPrincipal)
         {
+            // Give this a valid value in the vProgram.  FIXME: Doing observably
+            // different things in the vProgram is unsound if we aren't careful
+            // and poor practice in general.  Once SVX supports passing
+            // configuration other than just a principal, use that instead.
+            if (redierct_uri1 == null)
+                redierct_uri1 = $"https://{rpPrincipal.name}/dummy";
+
             client_id = client_id1;
             redirect_uri = redierct_uri1;
             client_secret = client_secret1;
             AuthorizationEndpointUrl = AuthorizationEndpointUrl1;
             TokenEndpointUrl = TokenEndpointUrl1;
+
+            // This will allow the state to be exported in prod and will be
+            // reached in the vProgram to know that the redirect_uri principal
+            // is a trusted server.
+            SVX.VProgram_API.AssumeActsFor(GenericAuth.GenericAuthStandards.GetUrlTargetPrincipal(redirect_uri), rpPrincipal);
+
+            stateGenerator = new StateGenerator(rpPrincipal, stateKey);
         }
 
-        protected abstract Type ModelAuthorizationServerType { get; }
-        // Get the content for Program.cs in the VProgram.
-        protected abstract string VProgramMainContent { get; }
+        protected abstract ModelAuthorizationServer CreateModelAuthorizationServer();
+
+        // This is a little arbitrary.  When we sort out how to pass
+        // configuration to participants, it would be a good opportunity to get
+        // rid of this.
+        protected sealed override SVX.ParticipantId idpParticipantId =>
+            SVX.ParticipantId.Of(CreateModelAuthorizationServer());
 
         /*** Methods about AuthorizationRequest ***/
-        public abstract AuthorizationRequest createAuthorizationRequest(SVX.SVX_MSG inputMSG, string SVAuthSessionID);
-        public AuthorizationRequest _createAuthorizationRequest(SVX.SVX_MSG inputMSG,string SVAuthSessionID)
-        {
-            var outputMSG = createAuthorizationRequest(inputMSG, SVAuthSessionID);
-            SVX.SVX_Ops.recordme(this, inputMSG, outputMSG);
-            return outputMSG;
-        }
-        public abstract string /*Uri*/ marshalAuthorizationRequest(AuthorizationRequest _AuthorizationRequest);
+        public abstract AuthorizationRequest createAuthorizationRequest(SVX.PrincipalFacet client);
+        public abstract string /*Uri*/ marshalAuthorizationRequest(AuthorizationRequest authorizationRequest);
 
         /*** Methods about AccessTokenRequest ***/
         protected virtual Type LoginCallbackRequestType { get { return typeof(AuthorizationResponse); } }
-        public virtual AccessTokenRequest createAccessTokenRequest(SVX.SVX_MSG inputMSG) { return null; }
-        public AccessTokenRequest _createAccessTokenRequest(SVX.SVX_MSG inputMSG)
-        {
-            var outputMSG = this.createAccessTokenRequest(inputMSG);
-            SVX.SVX_Ops.recordme(this, inputMSG, outputMSG);
-            return outputMSG;
-        }
-        public virtual HttpRequestMessage marshalAccessTokenRequest(AccessTokenRequest _AccessTokenRequest) { return null; }
+        public virtual AccessTokenRequest createAccessTokenRequest(AuthorizationResponse authorizationResponse) { return null; }
+        public virtual HttpRequestMessage marshalAccessTokenRequest(AccessTokenRequest accessTokenRequest) { return null; }
 
         /*** Methods about UserProfileRequest ***/
         protected virtual Type AccessTokenResponseType { get { return typeof(AccessTokenResponse); } }
-        public virtual UserProfileRequest createUserProfileRequest(SVX.SVX_MSG inputMSG) { return null; } 
-        public UserProfileRequest _createUserProfileRequest(SVX.SVX_MSG inputMSG)
-        {
-            var outputMSG = this.createUserProfileRequest(inputMSG);
-            // The input is the AccessTokenResponse, which is server-to-server.
-            SVX.SVX_Ops.recordme(this, inputMSG, outputMSG, false, true);
-            return outputMSG;
-        }
-        public virtual HttpRequestMessage marshalUserProfileRequest(UserProfileRequest _UserProfileRequest) { return null; }
+        public virtual UserProfileRequest createUserProfileRequest(AccessTokenResponse accessTokenResponse) { return null; }
+        public virtual HttpRequestMessage marshalUserProfileRequest(UserProfileRequest userProfileRequest) { return null; }
 
         /*** Methods about Conclusion ***/
         protected virtual Type UserProfileResponseType { get { return typeof(UserProfileResponse); } }
-        public abstract GenericAuth.AuthenticationConclusion createConclusion(SVX.SVX_MSG inputMSG);
-        public GenericAuth.AuthenticationConclusion _createConclusion(SVX.SVX_MSG inputMSG)
-        {
-            var outputMSG = this.createConclusion(inputMSG);
-            // The input is the UserProfileResponse, which is server-to-server.
-            //
-            // The conclusion is consumed locally.  I think treating it as
-            // signed will give the right result. ~ t-mattmc@microsoft.com 2016-06-06
-            SVX.SVX_Ops.recordme(this, inputMSG, outputMSG, true, true);
-            return outputMSG;
-        }
+        // conclusion.authenticatedClient should be set to authorizationResponse.SVX_sender.
+        // The arguments must be passed in this order for SVX to detect that
+        // userProfileResponse resulted from a computation on authorizationResponse.
+        public abstract GenericAuth.AuthenticationConclusion createConclusion(
+            AuthorizationResponse authorizationResponse, UserProfileResponse userProfileResponse);
 
         /*************** Start defining OAuth flows ************************/
-        public Task Login_StartAsync(HttpContext context)
+        public Task Login_StartAsync(HttpContext httpContext)
         {
-            SVX.SVX_MSG inputMSG = new SVX.SVX_MSG();
-            // This message should never contain meaningful data.
-            //JsonConvert.DeserializeObject<SVX.SVX_MSG>(Utils.ReadStream(context.Request.Body));
-            string SVAuthSessionID=Utils.SetNewSVAuthSessionIDHeader(context);
-            var _AuthorizationRequest = _createAuthorizationRequest(inputMSG, SVAuthSessionID);
+            var context = new SVAuthRequestContext(SVX_Principal, httpContext);
+
+            // The SymT doesn't actually get used, but why not.
+            var _AuthorizationRequest = SVX.SVX_Ops.Call(createAuthorizationRequest, context.client);
+
+            // NOTE: We are assuming that the target URL used by
+            // marshalAuthorizationRequest belongs to the principal
+            // idpParticipantId.principal.  We haven't extended SVX enforcement
+            // that far yet.
+            messageStructures.authorizationRequest.Export(_AuthorizationRequest, context.client, idpParticipantId.principal);
+            _AuthorizationRequest.SVX_serializeSymT = false;
             var rawReq = marshalAuthorizationRequest(_AuthorizationRequest);
-            context.Response.Redirect(rawReq);
+            context.http.Response.Redirect(rawReq);
 
             return Task.CompletedTask;
         }
-        public virtual async Task AuthorizationCodeFlow_Login_CallbackAsync(HttpContext context)
+        public virtual async Task AuthorizationCodeFlow_Login_CallbackAsync(HttpContext httpContext)
         {
             Trace.Write("AuthorizationCodeFlow_Login_CallbackAsync");
+            var context = new SVAuthRequestContext(SVX_Principal, httpContext);
+            var idp = CreateModelAuthorizationServer();
+
+            // See if any subclasses need us to use their special
+            // AuthorizationRequest subclass.
+            var dummyAuthorizationRequest = new AuthorizationRequest();
 
             // This design is following the original Auth.JS as closely as
             // possible.  Arguably, we should give concrete subclasses full
@@ -255,36 +340,272 @@ namespace SVAuth.OAuth20
             // parseHttpMessage supports both requests (query) and responses,
             // but here we know which is which.
             // ~ t-mattmc@microsoft.com 2016-06-01
-            SVX.SVX_MSG inputMSG = (SVX.SVX_MSG)Utils.ObjectFromQuery(
-                context.Request.Query, LoginCallbackRequestType);
-            var _AccessTokenRequest = _createAccessTokenRequest(inputMSG);
-            var rawReq = marshalAccessTokenRequest(_AccessTokenRequest);
-            var RawAccessTokenResponse = await SVX.Utils.PerformHttpRequestAsync(rawReq);
+            var authorizationResponse = (AuthorizationResponse)Utils.ObjectFromQuery(
+                context.http.Request.Query, LoginCallbackRequestType);
+
+            /* UNSOLVED PROBLEM: We are assuming that if we determine that the
+             * incoming message is from a trusted producer (which will be the
+             * case for the LoginXSRFPrevention property after we verify the
+             * state), then it actually came from the code endpoint.  This
+             * should be a safe assumption as long as we don't use the state
+             * generator for anything other than requests to the code endpoint
+             * and the IdP doesn't do anything with the state other than send it
+             * right back, but SVX currently provides no way to verify this
+             * reasoning.
+             */
+            idp.FakeCodeEndpoint(dummyAuthorizationRequest, authorizationResponse);
+
+            messageStructures.authorizationResponse.Import(authorizationResponse,
+                SVX.PrincipalFacet.GenerateNew(SVX_Principal),  // unknown producer
+                context.client);
+
+            var accessTokenRequest = SVX.SVX_Ops.Call(createAccessTokenRequest, authorizationResponse);
+
+            messageStructures.accessTokenRequest.Export(accessTokenRequest, idp.SVX_Principal, null);
+            accessTokenRequest.SVX_serializeSymT = false;
+            var rawAccessTokenRequest = marshalAccessTokenRequest(accessTokenRequest);
+            var rawAccessTokenResponse = await Utils.PerformHttpRequestAsync(rawAccessTokenRequest);
             Trace.Write("Got AccessTokenResponse");
+            var accessTokenResponse = (AccessTokenResponse)JsonConvert.DeserializeObject(
+                Utils.ReadContent(rawAccessTokenResponse.Content), AccessTokenResponseType);
+            idp.FakeTokenEndpoint(accessTokenRequest, accessTokenResponse);
+            messageStructures.accessTokenResponse.ImportDirectResponse(accessTokenResponse, idp.SVX_Principal, SVX_Principal);
 
-            SVX.SVX_MSG inputMSG2 = (SVX.SVX_MSG)JsonConvert.DeserializeObject(
-                Utils.ReadContent(RawAccessTokenResponse.Content), AccessTokenResponseType);
-            // TODO: Figure out the correct receiver and method name.
-            SVX.SVX_Ops.recordCustom(ModelAuthorizationServerType, _AccessTokenRequest, inputMSG2,
-                nameof(AuthorizationServer.TokenEndpoint), "AS", false, false);
-            var _UserProfileRequest = _createUserProfileRequest(inputMSG2);
-            var rawReq2 = marshalUserProfileRequest(_UserProfileRequest);
-            var RawUserProfileResponse = await SVX.Utils.PerformHttpRequestAsync(rawReq2);
+            var userProfileRequest = SVX.SVX_Ops.Call(createUserProfileRequest, accessTokenResponse);
+
+            messageStructures.userProfileRequest.Export(userProfileRequest, idp.SVX_Principal, null);
+            userProfileRequest.SVX_serializeSymT = false;
+            var rawUserProfileRequest = marshalUserProfileRequest(userProfileRequest);
+            var rawUserProfileResponse = await Utils.PerformHttpRequestAsync(rawUserProfileRequest);
             Trace.Write("Got UserProfileResponse");
+            var userProfileResponse = (UserProfileResponse)JsonConvert.DeserializeObject(
+                Utils.ReadContent(rawUserProfileResponse.Content), UserProfileResponseType);
+            idp.FakeUserProfileEndpoint(userProfileRequest, userProfileResponse);
+            messageStructures.userProfileResponse.ImportDirectResponse(userProfileResponse, idp.SVX_Principal, SVX_Principal);
 
-            SVX.SVX_MSG inputMSG3 = (SVX.SVX_MSG)JsonConvert.DeserializeObject(
-                Utils.ReadContent(RawUserProfileResponse.Content), UserProfileResponseType);
-            SVX.SVX_Ops.recordCustom(ModelAuthorizationServerType, _UserProfileRequest, inputMSG3,
-                nameof(AuthorizationServer.UserProfileEndpoint), "AS", false, false);
-            var conclusion = _createConclusion(inputMSG3);
+            var conclusion = SVX.SVX_Ops.Call(createConclusion, authorizationResponse, userProfileResponse);
 
-            SVX.VProgramGenerator.Program_cs = VProgramMainContent;
             await AuthenticationDone(conclusion, context);
         }
     }
 
-    public abstract class AuthorizationServer : GenericAuth.AS
+    public class AuthorizationCodeParams
     {
+        public string userID;
+        public string redirect_uri;
+    }
+
+    public class AuthorizationCodeGenerator : SVX.SecretGenerator<AuthorizationCodeParams>
+    {
+        readonly SVX.Principal idpPrincipal;
+
+        // Since this isn't a MessagePayloadSecretGenerator used with "verify on
+        // import", we don't have to worry about it having a default constructor
+        // for the time being, so we can do this, which leaves a little less
+        // boilerplate in concrete model IdPs than subclassing
+        // AuthorizationCodeGenerator and overriding a propertly.
+        public AuthorizationCodeGenerator(SVX.Principal idpPrincipal)
+        {
+            this.idpPrincipal = idpPrincipal;
+        }
+
+        protected override SVX.PrincipalHandle[] GetReaders(object theParams)
+        {
+            var params2 = (AuthorizationCodeParams)theParams;
+            return new SVX.Principal[] {
+                idpPrincipal,
+                GenericAuth.GenericAuthStandards.GetUrlTargetPrincipal(params2.redirect_uri),
+                GenericAuth.GenericAuthStandards.GetIdPUserPrincipal(idpPrincipal, params2.userID),
+            };
+        }
+
+        // Generate and Verify are called only by model IdP methods that are
+        // executed only in the vProgram, so these are not reached.
+
+        protected override string RawGenerate(AuthorizationCodeParams theParams)
+        {
+            throw new NotImplementedException();
+        }
+
+        protected override void RawVerify(AuthorizationCodeParams theParams, string secretValue)
+        {
+            throw new NotImplementedException();
+        }
+    }
+
+    public class AccessTokenParams
+    {
+        public string userID;
+    }
+
+    public class AccessTokenGenerator : SVX.TokenGenerator<AccessTokenParams>
+    {
+        // Ditto AuthorizationCodeGenerator.
+
+        protected override string RawGenerate(AccessTokenParams theParams)
+        {
+            throw new NotImplementedException();
+        }
+
+        protected override void RawVerify(AccessTokenParams theParams, string tokenValue)
+        {
+            throw new NotImplementedException();
+        }
+    }
+
+    // This class is not designed at this point to serve as a base for real
+    // authorization server implementations.
+    public abstract class ModelAuthorizationServer : GenericAuth.AS
+    {
+        // Make members overridable on first need...
+
+        // Lazy to avoid running initialization code in the vProgram.
+        MessageStructures messageStructures_;
+        MessageStructures messageStructures
+        {
+            get
+            {
+                if (messageStructures_ == null)
+                    messageStructures_ = new MessageStructures(SVX_Principal);
+                return messageStructures_;
+            }
+        }
+
+        readonly AuthorizationCodeGenerator authorizationCodeGenerator;
+        readonly AccessTokenGenerator accessTokenGenerator = new AccessTokenGenerator();
+
+        public ModelAuthorizationServer(SVX.Principal idpPrincipal)
+            : base(idpPrincipal)
+        {
+            // Initialization order restriction
+            authorizationCodeGenerator = new AuthorizationCodeGenerator(SVX_Principal);
+        }
+
+        public class IdPAuthenticationEntry : SVX.SVX_MSG
+        {
+            public SVX.PrincipalHandle authenticatedClient;
+            public string userID;
+        }
+
+        public void FakeCodeEndpoint(AuthorizationRequest req, AuthorizationResponse resp)
+        {
+            // XXX: Do we need to check that req.response_type == "code"?
+            // Currently, as per the comment in
+            // AuthorizationCodeFlow_Login_CallbackAsync, FakeCodeEndpoint only
+            // needs to handle the kinds of requests actually made by RP, which
+            // request a code.  We don't care about the value of
+            // req.response_type in its own right.
+
+            var producer = SVX.PrincipalFacet.GenerateNew(SVX_Principal);
+            var client = SVX.PrincipalFacet.GenerateNew(SVX_Principal);
+
+            messageStructures.authorizationRequest.FakeImport(req, producer, client);
+
+            var idpConc = new IdPAuthenticationEntry();  // Nondet
+            SVX.SVX_Ops.FakeCall(SVX_ConcludeClientAuthentication, idpConc, idpConc);
+
+            SVX.SVX_Ops.FakeCall(SVX_MakeAuthorizationResponse, req, idpConc, resp);
+
+            messageStructures.authorizationResponse.FakeExport(resp);
+        }
+
+        // Write lambda by hand because all compiler-generated classes are
+        // currently excluded from decompilation of method bodies by CCI.
+        class SignedInDeclarer
+        {
+            internal ModelAuthorizationServer outer;
+            internal IdPAuthenticationEntry entry;
+            internal void Declare()
+            {
+                outer.SignedInPredicate.Declare(SVX.VProgram_API.UnderlyingPrincipal(entry.authenticatedClient), entry.userID);
+            }
+        }
+
+        public IdPAuthenticationEntry SVX_ConcludeClientAuthentication(IdPAuthenticationEntry entry)
+        {
+            var d = new SignedInDeclarer { outer = this, entry = entry };
+            SVX.SVX_Ops.Ghost(d.Declare);
+            SVX.VProgram_API.AssumeActsFor(entry.authenticatedClient,
+                GenericAuth.GenericAuthStandards.GetIdPUserPrincipal(SVX_Principal, entry.userID));
+            // Reuse the message... Should be able to get away with it.
+            return entry;
+        }
+
+        public AuthorizationResponse SVX_MakeAuthorizationResponse(AuthorizationRequest req, IdPAuthenticationEntry idpConc)
+        {
+            // In the real CodeEndpoint, we would request an
+            // IdPAuthenticationEntry for req.SVX_sender, but SVX doesn't know
+            // that, so we have to do a concrete check.
+            SVX.VProgram_API.Assert(req.SVX_sender == idpConc.authenticatedClient);
+
+            // Copy/paste: [With this expression inlined below, BCT silently mistranslated the code.]
+            var theParams = new AuthorizationCodeParams
+            {
+                redirect_uri = req.redirect_uri,
+                userID = idpConc.userID
+            };
+            var authorizationCode = authorizationCodeGenerator.Generate(theParams, SVX_Principal);
+
+            return new AuthorizationResponse
+            {
+                code = authorizationCode,
+                state = req.state
+            };
+        }
+
+        public void FakeTokenEndpoint(AccessTokenRequest req, AccessTokenResponse resp)
+        {
+            // XXX: Anything we can do about this boilerplate?
+            var producer = SVX.PrincipalFacet.GenerateNew(SVX_Principal);
+            var client = SVX.PrincipalFacet.GenerateNew(SVX_Principal);
+
+            messageStructures.accessTokenRequest.FakeImport(req, producer, client);
+            SVX.SVX_Ops.FakeCall(SVX_MakeAccessTokenResponse, req, (AuthorizationCodeParams)null, resp);
+            messageStructures.accessTokenResponse.FakeExportDirectResponse(resp, producer);
+        }
+
+        public virtual AccessTokenResponse SVX_MakeAccessTokenResponse(AccessTokenRequest req, AuthorizationCodeParams codeParamsHint)
+        {
+            // We should only get here with req.grant_type ==
+            // "authorization_code", so we don't have to worry about modeling
+            // what IdP does in any other case.  Let us know if this isn't true.
+            Contract.Assert(req.grant_type == "authorization_code");
+
+            authorizationCodeGenerator.Verify(codeParamsHint, req.code);
+
+            if (req.redirect_uri != codeParamsHint.redirect_uri)
+                throw new Exception("Authorization code RP mismatch");
+
+            var tokenParams = new AccessTokenParams
+            {
+                userID = codeParamsHint.userID
+            };
+            var token = accessTokenGenerator.Generate(tokenParams);
+            return new AccessTokenResponse
+            {
+                access_token = token
+            };
+        }
+
+        public void FakeUserProfileEndpoint(UserProfileRequest req, UserProfileResponse resp)
+        {
+            var producer = SVX.PrincipalFacet.GenerateNew(SVX_Principal);
+            var client = SVX.PrincipalFacet.GenerateNew(SVX_Principal);
+
+            messageStructures.userProfileRequest.FakeImport(req, producer, client);
+            SVX.SVX_Ops.FakeCall(SVX_MakeUserProfileResponse, req, (AccessTokenParams)null, resp);
+            messageStructures.userProfileResponse.FakeExportDirectResponse(resp, producer);
+        }
+
+        public abstract UserProfileResponse CreateUserProfileResponse(string userID);
+
+        public UserProfileResponse SVX_MakeUserProfileResponse(UserProfileRequest req, AccessTokenParams tokenParamsHint)
+        {
+            accessTokenGenerator.Verify(tokenParamsHint, req.access_token);
+            return CreateUserProfileResponse(tokenParamsHint.userID);
+        }
+
+#if false
         static NondetOAuth20 NondetOAuth20;
         public Dictionary<string, AuthorizationCodeEntry> AuthorizationCodes = new Dictionary<string, AuthorizationCodeEntry>();
         public Dictionary<string, AccessTokenEntry> AccessTokens = new Dictionary<string, AccessTokenEntry>();
@@ -351,8 +672,11 @@ namespace SVAuth.OAuth20
         public abstract ID_Claim get_ID_Claim_From_Authorization_Request(AuthorizationRequest req);
         public abstract string createAccessToken(AuthorizationCodeEntry AuthorizationCodeEntry);
         public abstract UserProfileResponse createUserProfileResponse(ID_Claim ID_Claim);
+#endif
+
     }
 
+#if false
     public interface NondetOAuth20 : GenericAuth.Nondet_Base
     {
         int Int();
@@ -361,4 +685,5 @@ namespace SVAuth.OAuth20
         SVX.SVX_MSG SVX_MSG();
         AuthorizationCodeEntry AuthorizationCodeEntry();
     }
+#endif
 }
