SVAuth/ServiceProviders/Facebook/Facebook.cs
@@ -21,7 +21,7 @@ namespace SVAuth.ServiceProviders.Facebook
     {
         public string type;
     }
-    public class FBAuthConclusion : GenericAuth.AuthenticationConclusion
+    public class FBUserProfile : GenericAuth.UserProfile
     {
         public string Email;
         public string FullName;
@@ -34,6 +34,7 @@ namespace SVAuth.ServiceProviders.Facebook
         public string email;
     }
 
+#if false
     public class ID_Claim : OAuth20.ID_Claim
     {
        public string email, FB_ID, FullName;
@@ -49,64 +50,82 @@ namespace SVAuth.ServiceProviders.Facebook
             }
         }
     }
+#endif
     public class Facebook_RP : OAuth20.Client
     {
         public string UserProfileUrl;
-        public Facebook_RP(string client_id1 = null, string redierct_uri1 = null, string client_secret1 = null, string AuthorizationEndpointUrl1 = null, string TokenEndpointUrl1 = null, string UserProfileUrl1 = null)
-        : base(client_id1, redierct_uri1, client_secret1, AuthorizationEndpointUrl1, TokenEndpointUrl1)
+        public Facebook_RP(SVX.Principal rpPrincipal,
+            string client_id1 = null, string redierct_uri1 = null, string client_secret1 = null,
+            string AuthorizationEndpointUrl1 = null, string TokenEndpointUrl1 = null, string UserProfileUrl1 = null,
+            string stateKey = null)
+        : base(rpPrincipal, client_id1, redierct_uri1, client_secret1, AuthorizationEndpointUrl1, TokenEndpointUrl1, stateKey)
         {
             UserProfileUrl = UserProfileUrl1;
         }
 
-        protected override Type ModelAuthorizationServerType => typeof(Facebook_IdP_Default);
-        protected override string VProgramMainContent => File.ReadAllText("ServiceProviders/Facebook/VProgram.cs");
+        protected override OAuth20.ModelAuthorizationServer CreateModelAuthorizationServer() =>
+            new Facebook_IdP_Default(Facebook_IdP_Default.facebookPrincipal);
+
+        // Very little of this is Facebook-specific.  Consider moving it to
+        // OAuth20.  (Exception: it's unclear if "user profile" is an OAuth20
+        // concept at all, so maybe the entirety of that should move to Facebook
+        // with only a hook remaining in OAuth20.)
 
         /*** implementing the methods for AuthorizationRequest ***/
-        public override OAuth20.AuthorizationRequest createAuthorizationRequest(SVX.SVX_MSG inputMSG, string SVAuthSessionID)
+        public override OAuth20.AuthorizationRequest createAuthorizationRequest(SVX.PrincipalFacet client)
         {
-            FBAuthorizationRequest _FBAuthorizationRequest = new FBAuthorizationRequest();
-            _FBAuthorizationRequest.client_id = client_id;      
-            _FBAuthorizationRequest.response_type = "code";
-            _FBAuthorizationRequest.scope = "user_about_me email";
-            _FBAuthorizationRequest.redirect_uri = redirect_uri;
-            _FBAuthorizationRequest.type = "web_server";
-            return _FBAuthorizationRequest;
+            var authorizationRequest = new FBAuthorizationRequest();
+            authorizationRequest.client_id = client_id;      
+            authorizationRequest.response_type = "code";
+            authorizationRequest.scope = "user_about_me email";
+            authorizationRequest.redirect_uri = redirect_uri;
+            authorizationRequest.type = "web_server";
+            var stateParams = new OAuth20.StateParams
+            {
+                client = client,
+                idpPrincipal = idpParticipantId.principal
+            };
+            authorizationRequest.state = stateGenerator.Generate(stateParams, SVX_Principal);
+            return authorizationRequest;
         }
-        public override string marshalAuthorizationRequest(OAuth20.AuthorizationRequest _FBAuthorizationRequest)
+        public override string marshalAuthorizationRequest(OAuth20.AuthorizationRequest authorizationRequest)
         {
-            return AuthorizationEndpointUrl + "?" + Utils.ObjectToUrlEncodedString(_FBAuthorizationRequest);
+            return AuthorizationEndpointUrl + "?" + Utils.ObjectToUrlEncodedString(authorizationRequest);
         }
 
         /*** implementing the methods for AccessTokenRequest ***/
-        public override OAuth20.AccessTokenRequest createAccessTokenRequest(SVX.SVX_MSG inputMSG)
+        public override OAuth20.AccessTokenRequest createAccessTokenRequest(OAuth20.AuthorizationResponse authorizationResponse)
         {
+            var stateParams = new OAuth20.StateParams
+            {
+                client = authorizationResponse.SVX_sender,
+                idpPrincipal = idpParticipantId.principal
+            };
+            stateGenerator.Verify(stateParams, authorizationResponse.state);
+
             OAuth20.AccessTokenRequest _AccessTokenRequest = new OAuth20.AccessTokenRequest();
             //Facebook's access token request doesn't need "grant_type=authorization_code". 
             //See https://developers.facebook.com/docs/facebook-login/manually-build-a-login-flow
             _AccessTokenRequest.client_id = client_id;
-            _AccessTokenRequest.code = ((OAuth20.AuthorizationResponse)inputMSG).code;
+            _AccessTokenRequest.code = authorizationResponse.code;
             _AccessTokenRequest.redirect_uri = redirect_uri;
             _AccessTokenRequest.client_secret = client_secret;
             return _AccessTokenRequest;
         }
 
-        public override HttpRequestMessage marshalAccessTokenRequest(OAuth20.AccessTokenRequest _AccessTokenRequest)
+        public override HttpRequestMessage marshalAccessTokenRequest(OAuth20.AccessTokenRequest accessTokenRequest)
         {
-            // TODO (t-mattmc@microsoft.com): Replace with ObjectToForm once we confirm whether
-            // the grant_type field should be included?
-            var RawRequestUrl = TokenEndpointUrl + "?client_id=" + _AccessTokenRequest.client_id + "&redirect_uri=" + _AccessTokenRequest.redirect_uri
-                + "&client_secret=" + _AccessTokenRequest.client_secret + "&code=" + _AccessTokenRequest.code;
+            var RawRequestUrl = TokenEndpointUrl + "?" + Utils.ObjectToUrlEncodedString(accessTokenRequest);
             return new HttpRequestMessage(HttpMethod.Get, RawRequestUrl);
         }
 
         /*** implementing the methods for UserProfileRequest ***/
-        public override OAuth20.UserProfileRequest createUserProfileRequest(SVX.SVX_MSG inputMSG)
+        public override OAuth20.UserProfileRequest createUserProfileRequest(OAuth20.AccessTokenResponse accessTokenResponse)
         {
-            OAuth20.UserProfileRequest _UserProfileRequest = new OAuth20.UserProfileRequest();
-            //System.Diagnostics.Contracts.Contract.Assert(false);
-            _UserProfileRequest.access_token = ((OAuth20.AccessTokenResponse)inputMSG).access_token;
-            _UserProfileRequest.fields = "name,email";
-            return _UserProfileRequest;
+            OAuth20.UserProfileRequest userProfileRequest = new OAuth20.UserProfileRequest();
+            userProfileRequest.access_token = accessTokenResponse.access_token;
+            userProfileRequest.fields = "name,email";
+            return userProfileRequest;
         }
 
         public override HttpRequestMessage marshalUserProfileRequest(OAuth20.UserProfileRequest _UserProfileRequest)
@@ -117,32 +136,41 @@ namespace SVAuth.ServiceProviders.Facebook
 
         /*** implementing the methods for AuthenticationConclusion ***/
         protected override Type UserProfileResponseType { get { return typeof(FBUserProfileResponse); } }
-        public override GenericAuth.AuthenticationConclusion createConclusion(SVX.SVX_MSG inputMSG)
+        public override GenericAuth.AuthenticationConclusion createConclusion(
+            OAuth20.AuthorizationResponse authorizationResponse,
+            OAuth20.UserProfileResponse userProfileResponse)
         {
-            var _FBAuthConclusion = new FBAuthConclusion();
-            _FBAuthConclusion.UserID = ((FBUserProfileResponse)inputMSG).email;
-            _FBAuthConclusion.Email = ((FBUserProfileResponse)inputMSG).email;
-            _FBAuthConclusion.FB_ID = ((FBUserProfileResponse)inputMSG).id;
-            _FBAuthConclusion.FullName = ((FBUserProfileResponse)inputMSG).name;
-            return _FBAuthConclusion;
+            var fbUserProfileResponse = (FBUserProfileResponse)userProfileResponse;
+            var conclusion = new GenericAuth.AuthenticationConclusion();
+            conclusion.authenticatedClient = authorizationResponse.SVX_sender;
+            var fbUserProfile = new FBUserProfile();
+            fbUserProfile.UserID = fbUserProfileResponse.email;
+            fbUserProfile.Email = fbUserProfileResponse.email;
+            fbUserProfile.FB_ID = fbUserProfileResponse.id;
+            fbUserProfile.FullName = fbUserProfileResponse.name;
+            conclusion.userProfile = fbUserProfile;
+            return conclusion;
         }
 
         public static void Init(RouteBuilder routeBuilder)
         {
             var RP = new Facebook_RP(
+                Config.config.rpPrincipal,
                 Config.config.AppRegistration.Facebook.appId,
                 Config.config.agentRootUrl + "callback/Facebook",
                 Config.config.AppRegistration.Facebook.appSecret,
                 "https://www.facebook.com/v2.0/dialog/oauth",
                 "https://graph.facebook.com/v2.3/oauth/access_token",
-                "https://graph.facebook.com/v2.5/me"
+                "https://graph.facebook.com/v2.5/me",
+                Config.config.stateSecretKey
                 );
             routeBuilder.MapRoute("login/Facebook", RP.Login_StartAsync);
             routeBuilder.MapRoute("callback/Facebook", RP.AuthorizationCodeFlow_Login_CallbackAsync);
         }
     }
-    public class Facebook_IdP_Default : OAuth20.AuthorizationServer
+    public class Facebook_IdP_Default : OAuth20.ModelAuthorizationServer
     {
+#if false
         static OAuth20.NondetOAuth20 Nondet;
         //string UserID_Field_Name = "FB_ID";
 
@@ -183,12 +211,21 @@ namespace SVAuth.ServiceProviders.Facebook
                 setEntry("randomIdPSessID", "randomClientID", Nondet_FB.ID_Claim());
             }
         }
+#endif
 
-        public Facebook_IdP_Default()
+        public Facebook_IdP_Default(SVX.Principal idpPrincipal)
+            : base(idpPrincipal)
         {
+#if false
             IdentityRecords = new ID_Claims();
+#endif
+            // We only support facebookPrincipal.
+            Contract.Assert(idpPrincipal == facebookPrincipal);
         }
 
+        public static SVX.Principal facebookPrincipal = SVX.Principal.Of("facebook.com");
+
+#if false
         public override string createAccessToken(OAuth20.AuthorizationCodeEntry AuthorizationCodeEntry)
         {
             string AccessToken = Nondet.String();
@@ -229,21 +266,32 @@ namespace SVAuth.ServiceProviders.Facebook
             UserProfileResponse.name = ID_Claim.FullName;
             return UserProfileResponse;
         }
-
-        public override OAuth20.AccessTokenResponse TokenEndpoint(SVX.SVX_MSG req1)
+#endif
+        public override OAuth20.UserProfileResponse CreateUserProfileResponse(string userID)
         {
-            OAuth20.AccessTokenRequest req = (OAuth20.AccessTokenRequest)req1;
-            if (req == null) return null;
+            return new FBUserProfileResponse
+            {
+                id = SVX.VProgram_API.Nondet<string>(),
+                email = userID,
+                name = SVX.VProgram_API.Nondet<string>()
+            };
+        }
 
+        public override OAuth20.AccessTokenResponse SVX_MakeAccessTokenResponse(
+            OAuth20.AccessTokenRequest req, OAuth20.AuthorizationCodeParams codeParamsHint)
+        {
+#if false
             //Assumptions
             OAuth20.AuthorizationCodeEntry entry = AuthorizationCodes[req.code];
             //Assumption1: when facebook.com use the code to retrieve the client_id and the IdPSessionSecret, they are the ones for the SignInIdP
             System.Diagnostics.Contracts.Contract.Assume(entry.client_id == GenericAuth.GlobalObjects_base.SignInIdP_Req.Realm);
             System.Diagnostics.Contracts.Contract.Assume(entry.IdPSessionSecret == GenericAuth.GlobalObjects_base.SignInIdP_Req.IdPSessionSecret);
+#endif
             req.grant_type = "authorization_code";
-            return base.TokenEndpoint(req);
+            return base.SVX_MakeAccessTokenResponse(req, codeParamsHint);
         }
 
+#if false
         //Currently, the following two methods are essentially "unimplemented", because the SignInIdP call will be tossed away from the onion anyways. 
         //Perhaps there are some future scenarios in which these two methods need to be implemented. 
         public override GenericAuth.SignInIdP_Resp_SignInRP_Req Redir(string dest, GenericAuth.ID_Claim _ID_Claim)
@@ -254,6 +302,7 @@ namespace SVAuth.ServiceProviders.Facebook
         {
             return null;
         }
+#endif
     }
     /*
     public class Facebook_IdP_Email_As_UserID : Facebook_IdP_Default
