vProgram-skeleton/vProgram/run.bat
@@ -23,8 +23,8 @@ copy pub\runtimes\win\lib\netstandard1.3\*.dll pub
 
 REM With /e:1, BCT wasn't checking for an exception at the call site of SignInRP.
 REM I haven't investigated why yet. ~ t-mattmc@microsoft.com 2016-07-15
-call %SVAUTH_ROOT%\bytecodetranslator\Binaries\BytecodeTranslator.exe /e:2 /ib /whole /heap:splitFields /libpaths "@DOTNET_CORE_LIBPATH@" pub\vProgram.dll pub\SVAuth.dll pub\SVX_Common.dll
-call %SVAUTH_ROOT%\bytecodetranslator\corral\bin\Debug\BctCleanup.exe %model_name%.bpl %clean_name%.bpl /main:Program.Main /include:%SVAUTH_ROOT%\bytecodetranslator\collection_stubs.bpl /include:%SVAUTH_ROOT%\svx2_stubs.bpl
+call %SVAUTH_ROOT%\bytecodetranslator\Binaries\BytecodeTranslator.exe /e:2 /ib /whole /heap:splitFields /libpaths "@DOTNET_CORE_LIBPATH@" pub\vProgram.dll pub\SVAuth.dll pub\SVX.dll
+call %SVAUTH_ROOT%\bytecodetranslator\corral\bin\Debug\BctCleanup.exe %model_name%.bpl %clean_name%.bpl /main:Program.Main /include:%SVAUTH_ROOT%\bytecodetranslator\collection_stubs.bpl /include:%SVAUTH_ROOT%\svx_stubs.bpl
 call %SVAUTH_ROOT%\bytecodetranslator\corral\bin\Debug\corral.exe %clean_name%.bpl /printDataValues:1 /recursionBound:10 /k:1 /main:Program.Main /tryCTrace
 
 REM TODO: We want this for interactive use only.  Figure out how to conditionalize it.
